src/crypto/aes/aes-x64/proof.dfy
@@ -7,6 +7,8 @@ include "../../../arch/x64/vale64.i.dfy"
 include "../../../lib/util/dafny_wrappers.i.dfy"
 include "../ctr.s.dfy"
 include "../aes.s.dfy"
+include "../gcm3.s.dfy" 
+include "gcm_helpers.i.dfy"
 
 module proof {
 
@@ -15,6 +17,8 @@ import opened x64_def_s
 import opened types_s
 import opened dafny_wrappers_i
 import opened AESModule
-
+import opened GCMModule
+import opened GCMHelpers
 
 }
+
